\section{Product rule and chain rule of probability}
\subsection*{Product rule}
\par 
We define the conditional distribution of an r.v. using:
\[
    P(Y = y | X = y) = \dfrac{P(X = x, Y = y)}{P(X = x)}
\]
We can rearrange this equation to get:
\[
    P(x,y) = P(x)P(y|x)  
\]
\subsection*{Chain rule of probability}
\par 
By extending the product rule to $D$ variables, we obtain the chain rule of probability:
\[
    P(x_{1:D}) = P(x_1)P(x_2 | x_1) P(x_3 | x_1, x_2) \cdot \ldots \cdot P(x_D| x_{1:D-1})  
\]