\section{The exponential. Logarithms.}
Let's define exponential and logarithm:
\begin{definition}{(Exponential)}{}
    Let function $f: \ \R \to \R$ such that:
    \[
        f(x) = b^{kx},  
    \]
    with base $b > 0$ and constant $k$ is called the exponential function.
\end{definition}

\begin{definition}{(Logarithm)}{}
    A logarithm is an exponent which indicates to what power a base must be raised to produce a given number, i.e.:
    \[
        \begin{array}{cc}
            y = b^x & \text{ exponential form}\\
            x = \log_b y & \text{ logarithmic form}
        \end{array}  
    \]
\end{definition}

\begin{note}{}{}
    $x$ is the logarithm of $y$ to the base $b$, $\log_b y$ is the power to wich we have to raise $b$ to get $y$.
\end{note}

\par 
Common (Briggsian) logarithms (logarithms with base $10$). Notation:
\[
    \log_{10} y = \log y  
\]
\par 
Natural (Naperian) logarithms (logarithms with base $e$). Notation:
\[
    \log_e x = \ln x  
\]
\begin{theorema}{(Properties of exponents and logarithms)}{}
    \[
        \begin{array}{c} 
            b^m \cdot b^n \equiv b^{m+n} \\
            \dfrac{b^m}{b^n} \equiv b^{m-n}\\
            \left(b^m\right)^n\\[0.5cm] 
            \log_{b}(yz) = \log_b y + \log_b z\\
            \log_b (\dfrac{y}{z}) = \log_b y - \log_b z
        \end{array}
    \]
\end{theorema}
\begin{note}{}{}
    Other properties:
    \[
        \begin{array}{c}
            \ln x^y = y\cdot \ln x\\
            \ln e^x = x, \hspace*{0.5cm} e^{\ln x} = x\\
            \log_b a = \dfrac{\ln a}{\ln b} = \dfrac{\log a}{\log b}
        \end{array}  
    \]
\end{note}